Fix capitalizations

AutomataTheory/AutomataHist.lean
@@ -22,7 +22,7 @@ def AutomataHist (M : Automata A) (hist_init : Set H) (hist_next : M.State × H 
 
 variable (M : Automata A) (hist_init : Set H) (hist_next : M.State × H → A → Set H)
 
-theorem Automata_hist_inf_run_proj {as : ℕ → A} {ss : ℕ → M.State × H}
+theorem automata_hist_inf_run_proj {as : ℕ → A} {ss : ℕ → M.State × H}
     (h : InfRun (AutomataHist M hist_init hist_next) as ss) : InfRun M as (Prod.fst ∘ ss) := by
   constructor
   · have h' := h.1
@@ -33,21 +33,21 @@ theorem Automata_hist_inf_run_proj {as : ℕ → A} {ss : ℕ → M.State × H}
     simp [AutomataHist] at h'
     exact h'.1
 
-private def _MakeHist (as : ℕ → A) (ss : ℕ → M.State) (hs0 : H) (hs' : M.State × H → A -> H) : ℕ → H
+private def MakeHist (as : ℕ → A) (ss : ℕ → M.State) (hs0 : H) (hs' : M.State × H → A -> H) : ℕ → H
   | 0 => hs0
-  | k + 1 => hs' (ss k, _MakeHist as ss hs0 hs' k) (as k)
+  | k + 1 => hs' (ss k, MakeHist as ss hs0 hs' k) (as k)
 
-theorem Automata_hist_inf_run_exists {as : ℕ → A} {ss : ℕ → M.State}
+theorem automata_hist_inf_run_exists {as : ℕ → A} {ss : ℕ → M.State}
     (h_init : hist_init.Nonempty) (h_next : ∀ s a, (hist_next s a).Nonempty)
     (h : InfRun M as ss) : ∃ hs : ℕ → H, InfRun (AutomataHist M hist_init hist_next) as (fun k ↦ (ss k, hs k)) := by
   obtain ⟨hs0, h_hs0⟩ := h_init
   choose hs' h_hs' using h_next
-  let hs := _MakeHist M as ss hs0 hs'
+  let hs := MakeHist M as ss hs0 hs'
   use hs ; constructor
-  · simp [AutomataHist, _MakeHist, h.1, hs]
+  · simp [AutomataHist, MakeHist, h.1, hs]
     exact h_hs0
   · intro k
-    simp [AutomataHist, _MakeHist, hs, h.2 k]
+    simp [AutomataHist, MakeHist, hs, h.2 k]
     apply h_hs'
 
 end AutomataHist
